Regenerate the files

tests/coq/misc/Loops.v
@@ -70,8 +70,31 @@ Definition sum_with_shared_borrows (n : nat) (max : u32) : result u32 :=
   sum_with_shared_borrows_loop n max 0%u32 0%u32
 .
 
+(** [loops::sum_array]: loop 0:
+    Source: 'src/loops.rs', lines 50:0-58:1 *)
+Fixpoint sum_array_loop
+  (N : usize) (n : nat) (a : array u32 N) (i : usize) (s : u32) : result u32 :=
+  match n with
+  | O => Fail_ OutOfFuel
+  | S n1 =>
+    if i s< N
+    then (
+      i1 <- array_index_usize u32 N a i;
+      s1 <- u32_add s i1;
+      i2 <- usize_add i 1%usize;
+      sum_array_loop N n1 a i2 s1)
+    else Return s
+  end
+.
+
+(** [loops::sum_array]:
+    Source: 'src/loops.rs', lines 50:0-50:52 *)
+Definition sum_array (N : usize) (n : nat) (a : array u32 N) : result u32 :=
+  sum_array_loop N n a 0%usize 0%u32
+.
+
 (** [loops::clear]: loop 0:
-    Source: 'src/loops.rs', lines 52:0-58:1 *)
+    Source: 'src/loops.rs', lines 62:0-68:1 *)
 Fixpoint clear_loop
   (n : nat) (v : alloc_vec_Vec u32) (i : usize) : result (alloc_vec_Vec u32) :=
   match n with
@@ -92,14 +115,14 @@ Fixpoint clear_loop
 .
 
 (** [loops::clear]:
-    Source: 'src/loops.rs', lines 52:0-52:30 *)
+    Source: 'src/loops.rs', lines 62:0-62:30 *)
 Definition clear
   (n : nat) (v : alloc_vec_Vec u32) : result (alloc_vec_Vec u32) :=
   clear_loop n v 0%usize
 .
 
 (** [loops::List]
-    Source: 'src/loops.rs', lines 60:0-60:16 *)
+    Source: 'src/loops.rs', lines 70:0-70:16 *)
 Inductive List_t (T : Type) :=
 | List_Cons : T -> List_t T -> List_t T
 | List_Nil : List_t T
@@ -109,7 +132,7 @@ Arguments List_Cons { _ }.
 Arguments List_Nil { _ }.
 
 (** [loops::list_mem]: loop 0:
-    Source: 'src/loops.rs', lines 66:0-75:1 *)
+    Source: 'src/loops.rs', lines 76:0-85:1 *)
 Fixpoint list_mem_loop (n : nat) (x : u32) (ls : List_t u32) : result bool :=
   match n with
   | O => Fail_ OutOfFuel
@@ -122,13 +145,13 @@ Fixpoint list_mem_loop (n : nat) (x : u32) (ls : List_t u32) : result bool :=
 .
 
 (** [loops::list_mem]:
-    Source: 'src/loops.rs', lines 66:0-66:52 *)
+    Source: 'src/loops.rs', lines 76:0-76:52 *)
 Definition list_mem (n : nat) (x : u32) (ls : List_t u32) : result bool :=
   list_mem_loop n x ls
 .
 
 (** [loops::list_nth_mut_loop]: loop 0:
-    Source: 'src/loops.rs', lines 78:0-88:1 *)
+    Source: 'src/loops.rs', lines 88:0-98:1 *)
 Fixpoint list_nth_mut_loop_loop
   (T : Type) (n : nat) (ls : List_t T) (i : u32) :
   result (T * (T -> result (List_t T)))
@@ -155,7 +178,7 @@ Fixpoint list_nth_mut_loop_loop
 .
 
 (** [loops::list_nth_mut_loop]:
-    Source: 'src/loops.rs', lines 78:0-78:71 *)
+    Source: 'src/loops.rs', lines 88:0-88:71 *)
 Definition list_nth_mut_loop
   (T : Type) (n : nat) (ls : List_t T) (i : u32) :
   result (T * (T -> result (List_t T)))
@@ -164,7 +187,7 @@ Definition list_nth_mut_loop
 .
 
 (** [loops::list_nth_shared_loop]: loop 0:
-    Source: 'src/loops.rs', lines 91:0-101:1 *)
+    Source: 'src/loops.rs', lines 101:0-111:1 *)
 Fixpoint list_nth_shared_loop_loop
   (T : Type) (n : nat) (ls : List_t T) (i : u32) : result T :=
   match n with
@@ -181,14 +204,14 @@ Fixpoint list_nth_shared_loop_loop
 .
 
 (** [loops::list_nth_shared_loop]:
-    Source: 'src/loops.rs', lines 91:0-91:66 *)
+    Source: 'src/loops.rs', lines 101:0-101:66 *)
 Definition list_nth_shared_loop
   (T : Type) (n : nat) (ls : List_t T) (i : u32) : result T :=
   list_nth_shared_loop_loop T n ls i
 .
 
 (** [loops::get_elem_mut]: loop 0:
-    Source: 'src/loops.rs', lines 103:0-117:1 *)
+    Source: 'src/loops.rs', lines 113:0-127:1 *)
 Fixpoint get_elem_mut_loop
   (n : nat) (x : usize) (ls : List_t usize) :
   result (usize * (usize -> result (List_t usize)))
@@ -214,7 +237,7 @@ Fixpoint get_elem_mut_loop
 .
 
 (** [loops::get_elem_mut]:
-    Source: 'src/loops.rs', lines 103:0-103:73 *)
+    Source: 'src/loops.rs', lines 113:0-113:73 *)
 Definition get_elem_mut
   (n : nat) (slots : alloc_vec_Vec (List_t usize)) (x : usize) :
   result (usize * (usize -> result (alloc_vec_Vec (List_t usize))))
@@ -230,7 +253,7 @@ Definition get_elem_mut
 .
 
 (** [loops::get_elem_shared]: loop 0:
-    Source: 'src/loops.rs', lines 119:0-133:1 *)
+    Source: 'src/loops.rs', lines 129:0-143:1 *)
 Fixpoint get_elem_shared_loop
   (n : nat) (x : usize) (ls : List_t usize) : result usize :=
   match n with
@@ -245,7 +268,7 @@ Fixpoint get_elem_shared_loop
 .
 
 (** [loops::get_elem_shared]:
-    Source: 'src/loops.rs', lines 119:0-119:68 *)
+    Source: 'src/loops.rs', lines 129:0-129:68 *)
 Definition get_elem_shared
   (n : nat) (slots : alloc_vec_Vec (List_t usize)) (x : usize) :
   result usize
@@ -257,7 +280,7 @@ Definition get_elem_shared
 .
 
 (** [loops::id_mut]:
-    Source: 'src/loops.rs', lines 135:0-135:50 *)
+    Source: 'src/loops.rs', lines 145:0-145:50 *)
 Definition id_mut
   (T : Type) (ls : List_t T) :
   result ((List_t T) * (List_t T -> result (List_t T)))
@@ -266,13 +289,13 @@ Definition id_mut
 .
 
 (** [loops::id_shared]:
-    Source: 'src/loops.rs', lines 139:0-139:45 *)
+    Source: 'src/loops.rs', lines 149:0-149:45 *)
 Definition id_shared (T : Type) (ls : List_t T) : result (List_t T) :=
   Return ls
 .
 
 (** [loops::list_nth_mut_loop_with_id]: loop 0:
-    Source: 'src/loops.rs', lines 144:0-155:1 *)
+    Source: 'src/loops.rs', lines 154:0-165:1 *)
 Fixpoint list_nth_mut_loop_with_id_loop
   (T : Type) (n : nat) (i : u32) (ls : List_t T) :
   result (T * (T -> result (List_t T)))
@@ -299,7 +322,7 @@ Fixpoint list_nth_mut_loop_with_id_loop
 .
 
 (** [loops::list_nth_mut_loop_with_id]:
-    Source: 'src/loops.rs', lines 144:0-144:75 *)
+    Source: 'src/loops.rs', lines 154:0-154:75 *)
 Definition list_nth_mut_loop_with_id
   (T : Type) (n : nat) (ls : List_t T) (i : u32) :
   result (T * (T -> result (List_t T)))
@@ -313,7 +336,7 @@ Definition list_nth_mut_loop_with_id
 .
 
 (** [loops::list_nth_shared_loop_with_id]: loop 0:
-    Source: 'src/loops.rs', lines 158:0-169:1 *)
+    Source: 'src/loops.rs', lines 168:0-179:1 *)
 Fixpoint list_nth_shared_loop_with_id_loop
   (T : Type) (n : nat) (i : u32) (ls : List_t T) : result T :=
   match n with
@@ -331,14 +354,14 @@ Fixpoint list_nth_shared_loop_with_id_loop
 .
 
 (** [loops::list_nth_shared_loop_with_id]:
-    Source: 'src/loops.rs', lines 158:0-158:70 *)
+    Source: 'src/loops.rs', lines 168:0-168:70 *)
 Definition list_nth_shared_loop_with_id
   (T : Type) (n : nat) (ls : List_t T) (i : u32) : result T :=
   ls1 <- id_shared T ls; list_nth_shared_loop_with_id_loop T n i ls1
 .
 
 (** [loops::list_nth_mut_loop_pair]: loop 0:
-    Source: 'src/loops.rs', lines 174:0-195:1 *)
+    Source: 'src/loops.rs', lines 184:0-205:1 *)
 Fixpoint list_nth_mut_loop_pair_loop
   (T : Type) (n : nat) (ls0 : List_t T) (ls1 : List_t T) (i : u32) :
   result ((T * T) * (T -> result (List_t T)) * (T -> result (List_t T)))
@@ -372,7 +395,7 @@ Fixpoint list_nth_mut_loop_pair_loop
 .
 
 (** [loops::list_nth_mut_loop_pair]:
-    Source: 'src/loops.rs', lines 174:0-178:27 *)
+    Source: 'src/loops.rs', lines 184:0-188:27 *)
 Definition list_nth_mut_loop_pair
   (T : Type) (n : nat) (ls0 : List_t T) (ls1 : List_t T) (i : u32) :
   result ((T * T) * (T -> result (List_t T)) * (T -> result (List_t T)))
@@ -383,7 +406,7 @@ Definition list_nth_mut_loop_pair
 .
 
 (** [loops::list_nth_shared_loop_pair]: loop 0:
-    Source: 'src/loops.rs', lines 198:0-219:1 *)
+    Source: 'src/loops.rs', lines 208:0-229:1 *)
 Fixpoint list_nth_shared_loop_pair_loop
   (T : Type) (n : nat) (ls0 : List_t T) (ls1 : List_t T) (i : u32) :
   result (T * T)
@@ -407,7 +430,7 @@ Fixpoint list_nth_shared_loop_pair_loop
 .
 
 (** [loops::list_nth_shared_loop_pair]:
-    Source: 'src/loops.rs', lines 198:0-202:19 *)
+    Source: 'src/loops.rs', lines 208:0-212:19 *)
 Definition list_nth_shared_loop_pair
   (T : Type) (n : nat) (ls0 : List_t T) (ls1 : List_t T) (i : u32) :
   result (T * T)
@@ -416,7 +439,7 @@ Definition list_nth_shared_loop_pair
 .
 
 (** [loops::list_nth_mut_loop_pair_merge]: loop 0:
-    Source: 'src/loops.rs', lines 223:0-238:1 *)
+    Source: 'src/loops.rs', lines 233:0-248:1 *)
 Fixpoint list_nth_mut_loop_pair_merge_loop
   (T : Type) (n : nat) (ls0 : List_t T) (ls1 : List_t T) (i : u32) :
   result ((T * T) * ((T * T) -> result ((List_t T) * (List_t T))))
@@ -453,7 +476,7 @@ Fixpoint list_nth_mut_loop_pair_merge_loop
 .
 
 (** [loops::list_nth_mut_loop_pair_merge]:
-    Source: 'src/loops.rs', lines 223:0-227:27 *)
+    Source: 'src/loops.rs', lines 233:0-237:27 *)
 Definition list_nth_mut_loop_pair_merge
   (T : Type) (n : nat) (ls0 : List_t T) (ls1 : List_t T) (i : u32) :
   result ((T * T) * ((T * T) -> result ((List_t T) * (List_t T))))
@@ -464,7 +487,7 @@ Definition list_nth_mut_loop_pair_merge
 .
 
 (** [loops::list_nth_shared_loop_pair_merge]: loop 0:
-    Source: 'src/loops.rs', lines 241:0-256:1 *)
+    Source: 'src/loops.rs', lines 251:0-266:1 *)
 Fixpoint list_nth_shared_loop_pair_merge_loop
   (T : Type) (n : nat) (ls0 : List_t T) (ls1 : List_t T) (i : u32) :
   result (T * T)
@@ -489,7 +512,7 @@ Fixpoint list_nth_shared_loop_pair_merge_loop
 .
 
 (** [loops::list_nth_shared_loop_pair_merge]:
-    Source: 'src/loops.rs', lines 241:0-245:19 *)
+    Source: 'src/loops.rs', lines 251:0-255:19 *)
 Definition list_nth_shared_loop_pair_merge
   (T : Type) (n : nat) (ls0 : List_t T) (ls1 : List_t T) (i : u32) :
   result (T * T)
@@ -498,7 +521,7 @@ Definition list_nth_shared_loop_pair_merge
 .
 
 (** [loops::list_nth_mut_shared_loop_pair]: loop 0:
-    Source: 'src/loops.rs', lines 259:0-274:1 *)
+    Source: 'src/loops.rs', lines 269:0-284:1 *)
 Fixpoint list_nth_mut_shared_loop_pair_loop
   (T : Type) (n : nat) (ls0 : List_t T) (ls1 : List_t T) (i : u32) :
   result ((T * T) * (T -> result (List_t T)))
@@ -529,7 +552,7 @@ Fixpoint list_nth_mut_shared_loop_pair_loop
 .
 
 (** [loops::list_nth_mut_shared_loop_pair]:
-    Source: 'src/loops.rs', lines 259:0-263:23 *)
+    Source: 'src/loops.rs', lines 269:0-273:23 *)
 Definition list_nth_mut_shared_loop_pair
   (T : Type) (n : nat) (ls0 : List_t T) (ls1 : List_t T) (i : u32) :
   result ((T * T) * (T -> result (List_t T)))
@@ -540,7 +563,7 @@ Definition list_nth_mut_shared_loop_pair
 .
 
 (** [loops::list_nth_mut_shared_loop_pair_merge]: loop 0:
-    Source: 'src/loops.rs', lines 278:0-293:1 *)
+    Source: 'src/loops.rs', lines 288:0-303:1 *)
 Fixpoint list_nth_mut_shared_loop_pair_merge_loop
   (T : Type) (n : nat) (ls0 : List_t T) (ls1 : List_t T) (i : u32) :
   result ((T * T) * (T -> result (List_t T)))
@@ -571,7 +594,7 @@ Fixpoint list_nth_mut_shared_loop_pair_merge_loop
 .
 
 (** [loops::list_nth_mut_shared_loop_pair_merge]:
-    Source: 'src/loops.rs', lines 278:0-282:23 *)
+    Source: 'src/loops.rs', lines 288:0-292:23 *)
 Definition list_nth_mut_shared_loop_pair_merge
   (T : Type) (n : nat) (ls0 : List_t T) (ls1 : List_t T) (i : u32) :
   result ((T * T) * (T -> result (List_t T)))
@@ -582,7 +605,7 @@ Definition list_nth_mut_shared_loop_pair_merge
 .
 
 (** [loops::list_nth_shared_mut_loop_pair]: loop 0:
-    Source: 'src/loops.rs', lines 297:0-312:1 *)
+    Source: 'src/loops.rs', lines 307:0-322:1 *)
 Fixpoint list_nth_shared_mut_loop_pair_loop
   (T : Type) (n : nat) (ls0 : List_t T) (ls1 : List_t T) (i : u32) :
   result ((T * T) * (T -> result (List_t T)))
@@ -613,7 +636,7 @@ Fixpoint list_nth_shared_mut_loop_pair_loop
 .
 
 (** [loops::list_nth_shared_mut_loop_pair]:
-    Source: 'src/loops.rs', lines 297:0-301:23 *)
+    Source: 'src/loops.rs', lines 307:0-311:23 *)
 Definition list_nth_shared_mut_loop_pair
   (T : Type) (n : nat) (ls0 : List_t T) (ls1 : List_t T) (i : u32) :
   result ((T * T) * (T -> result (List_t T)))
@@ -624,7 +647,7 @@ Definition list_nth_shared_mut_loop_pair
 .
 
 (** [loops::list_nth_shared_mut_loop_pair_merge]: loop 0:
-    Source: 'src/loops.rs', lines 316:0-331:1 *)
+    Source: 'src/loops.rs', lines 326:0-341:1 *)
 Fixpoint list_nth_shared_mut_loop_pair_merge_loop
   (T : Type) (n : nat) (ls0 : List_t T) (ls1 : List_t T) (i : u32) :
   result ((T * T) * (T -> result (List_t T)))
@@ -655,7 +678,7 @@ Fixpoint list_nth_shared_mut_loop_pair_merge_loop
 .
 
 (** [loops::list_nth_shared_mut_loop_pair_merge]:
-    Source: 'src/loops.rs', lines 316:0-320:23 *)
+    Source: 'src/loops.rs', lines 326:0-330:23 *)
 Definition list_nth_shared_mut_loop_pair_merge
   (T : Type) (n : nat) (ls0 : List_t T) (ls1 : List_t T) (i : u32) :
   result ((T * T) * (T -> result (List_t T)))
